defeq refactor

SPos/Typing/Typing.lean
@@ -7,57 +7,80 @@ set_option hygiene false
 notation:40 "⊢" Γ:40 => WfCtx Γ
 notation:40 Γ:41 "∋" x:41 "∶" τ:41 => Lookup Γ x τ
 notation:40 Γ:41 "⊢" t:41 "≡" t':41 "∶" τ:41 => DefEq Γ t t' τ
+notation:40 Γ:41 "⊢" t:41 "∶" τ:41 => DefEq Γ t t τ
 
 inductive Lookup : Ctx n → Fin n → Tm n → Prop where
 | here  : Γ ∷ τ ∋ 0 ∶ ↑ τ
 | there : Γ ∋ n ∶ τ → Γ ∷ υ ∋ n.succ ∶ ↑ τ
 
--- Typed definitional equality is the ONLY term judgment; typing is its
--- diagonal (`WfTm` below is an abbreviation, not an inductive).
 mutual
 inductive WfCtx : Ctx n → Prop where
 | nil  : ⊢ ∅
-| cons : ⊢ Γ → Γ ⊢ τ ≡ τ ∶ 𝓤 ℓ → ⊢ Γ ∷ τ
+| cons : ⊢ Γ → Γ ⊢ τ ∶ 𝓤 ℓ → ⊢ Γ ∷ τ
+
+-- The idea is absuing structural rules to get the standard typing
+-- judgjments
 
 inductive DefEq : Ctx n → Tm n → Tm n → Tm n → Prop where
-| var   : ⊢ Γ → Γ ∋ x ∶ τ → Γ ⊢ # x ≡ # x ∶ τ
-| u     : ⊢ Γ → Γ ⊢ 𝓤 ℓ ≡ 𝓤 ℓ ∶ 𝓤 (ℓ + 1)
-| symm  : Γ ⊢ t ≡ t' ∶ τ → Γ ⊢ t' ≡ t ∶ τ
-| trans : Γ ⊢ t ≡ t' ∶ τ → Γ ⊢ t' ≡ t'' ∶ τ → Γ ⊢ t ≡ t'' ∶ τ
-| conv  : Γ ⊢ t ≡ t' ∶ τ → Γ ⊢ σ ≡ σ ∶ 𝓤 ℓ → Γ ⊢ τ ≡ σ ∶ 𝓤 ℓ → Γ ⊢ t ≡ t' ∶ σ
+-- Structual rules
+| symm  : Γ ⊢ t₁ ≡ t₂ ∶ τ
+        -----------------
+       → Γ ⊢ t₂ ≡ t₁ ∶ τ
+| trans : Γ ⊢ t₁ ≡ t₂ ∶ τ → Γ ⊢ t₂ ≡ t₃ ∶ τ
+        ------------------------------------
+       → Γ ⊢ t₁ ≡ t₃ ∶ τ
+-- Conversion
+| conv : Γ ⊢ t₁ ≡ t₂ ∶ τ₁ → Γ ⊢ τ₂ ∶ 𝓤 ℓ → Γ ⊢ τ₁ ≡ τ₂ ∶ 𝓤 ℓ
+       --------------------------------------------------------
+      → Γ ⊢ t₁ ≡ t₂ ∶ τ₂
+-- Variable
+| var : ⊢ Γ → Γ ∋ x ∶ τ
+      ------------------
+     → Γ ⊢ # x ∶ τ
+-- Universe
+| u : ⊢ Γ
+    ----------------------
+   → Γ ⊢ 𝓤 ℓ ∶ 𝓤 (ℓ + 1)
 -- Pi
-| pi  : Γ ⊢ τ ≡ τ' ∶ 𝓤 ℓ₁ → Γ ∷ τ ⊢ υ ≡ υ' ∶ 𝓤 ℓ₂ → Γ ⊢ Π τ υ ≡ Π τ' υ' ∶ 𝓤 (max ℓ₁ ℓ₂)
-| lam : Γ ∷ τ ⊢ σ ≡ σ ∶ 𝓤 ℓ' → Γ ⊢ τ ≡ τ' ∶ 𝓤 ℓ → Γ ∷ τ ⊢ t ≡ t' ∶ σ →
-        Γ ⊢ ƛ τ t ≡ ƛ τ' t' ∶ (Π τ σ)
-| app : Γ ⊢ t ≡ t' ∶ (Π τ σ) → Γ ⊢ m ≡ m' ∶ τ → Γ ⊢ t • m ≡ t' • m' ∶ σ [/ m ]
-| lamβ : Γ ⊢ τ ≡ τ ∶ 𝓤 ℓ → Γ ∷ τ ⊢ σ ≡ σ ∶ 𝓤 ℓ' → Γ ∷ τ ⊢ t ≡ t ∶ σ → Γ ⊢ m ≡ m ∶ τ →
-         Γ ⊢ (ƛ τ t) • m ≡ t [/ m ] ∶ σ [/ m ]
-| lamη : Γ ⊢ t ≡ t ∶ Π τ υ → Γ ⊢ t ≡ ƛ τ (↑ t) • # 0 ∶ Π τ υ
+| pi  : Γ ⊢ τ₁ ≡ τ₂ ∶ 𝓤 ℓ₁ → Γ ∷ τ₁ ⊢ υ₁ ≡ υ₂ ∶ 𝓤 ℓ₂
+      ------------------------------------------------
+     → Γ ⊢ Π τ₁ υ₁ ≡ Π τ₂ υ₂ ∶ 𝓤 (max ℓ₁ ℓ₂)
+-- Alecs(TODO): Figure out how to drop the well formedness of υ
+| lam : Γ ∷ τ₁ ⊢ υ ∶ 𝓤 ℓ' → Γ ⊢ τ₁ ≡ τ₂ ∶ 𝓤 ℓ → Γ ∷ τ₁ ⊢ t₁ ≡ t₂ ∶ υ
+      ----------------------------------------------------------------
+     → Γ ⊢ ƛ τ₁ t₁ ≡ ƛ τ₂ t₂ ∶ (Π τ₁ υ)
+| app : Γ ⊢ t₁ ≡ t₂ ∶ (Π τ υ) → Γ ⊢ m₁ ≡ m₂ ∶ τ
+      ------------------------------------------
+     → Γ ⊢ t₁ • m₁ ≡ t₂ • m₂ ∶ υ [/ m₁ ]
+| lamβ : Γ ⊢ τ ∶ 𝓤 ℓ → Γ ∷ τ ⊢ υ ∶ 𝓤 ℓ' → Γ ∷ τ ⊢ t ∶ υ → Γ ⊢ m ∶ τ
+       -----------------------------------------------------------------
+      → Γ ⊢ (ƛ τ t) • m ≡ t [/ m ] ∶ υ [/ m ]
+| lamη : Γ ⊢ t ∶ Π τ υ
+       -----------------------------------
+      → Γ ⊢ t ≡ ƛ τ (↑ t) • # 0 ∶ Π τ υ
 -- Identity
-| id : Γ ⊢ τ ≡ τ' ∶ 𝓤 ℓ → Γ ⊢ a ≡ a' ∶ τ → Γ ⊢ b ≡ b' ∶ τ →
-       Γ ⊢ Id τ a b ≡ Id τ' a' b' ∶ 𝓤 ℓ
-| reflId : Γ ⊢ τ ≡ τ' ∶ 𝓤 ℓ → Γ ⊢ a ≡ a' ∶ τ → Γ ⊢ refl τ a ≡ refl τ' a' ∶ Id τ a a
-| j {a : Tm n} :
-      Γ ⊢ τ ≡ τ ∶ 𝓤 ℓ₁ →
-      Γ ∷ τ ⊢ Id (↑ τ) (↑ a) # 0 ≡ Id (↑ τ) (↑ a) # 0 ∶ 𝓤 ℓ₁ →
-      Γ ∷ τ ∷ Id (↑ τ) (↑ a) # 0 ⊢ C ≡ C' ∶ 𝓤 ℓ →
-      Γ ⊢ d ≡ d' ∶ C [/ refl (↑ τ) (↑ a) ] [/ a ] →
-      Γ ⊢ p ≡ p' ∶ Id τ a b →
-      Γ ⊢ J C d p ≡ J C' d' p' ∶ C [/ ↑ p ] [/ b ]
-| jβ : Γ ⊢ τ ≡ τ ∶ 𝓤 ℓ₁ → Γ ⊢ a ≡ a ∶ τ →
-       Γ ∷ τ ⊢ Id (↑ τ) (↑ a) # 0 ≡ Id (↑ τ) (↑ a) # 0 ∶ 𝓤 ℓ₁ →
-       Γ ∷ τ ∷ Id (↑ τ) (↑ a) # 0 ⊢ C ≡ C ∶ 𝓤 ℓ →
-       Γ ⊢ d ≡ d ∶ C [/ refl (↑ τ) (↑ a) ] [/ a ] →
-       Γ ⊢ J C d (refl τ a) ≡ d ∶ C [/ refl (↑ τ) (↑ a) ] [/ a ]
+| id : Γ ⊢ τ₁ ≡ τ₂ ∶ 𝓤 ℓ → Γ ⊢ a₁ ≡ a₂ ∶ τ₁ → Γ ⊢ b₁ ≡ b₂ ∶ τ₁
+     ------------------------------------------------------------
+    → Γ ⊢ Id τ₁ a₁ b₁ ≡ Id τ₂ a₂ b₂ ∶ 𝓤 ℓ
+| refl : Γ ⊢ τ₁ ≡ τ₂ ∶ 𝓤 ℓ → Γ ⊢ a₁ ≡ a₂ ∶ τ₁
+       -------------------------------------------
+      → Γ ⊢ refl τ₁ a₁ ≡ refl τ₂ a₂ ∶ Id τ₁ a₁ a₁
+| j : {a : Tm n} → Γ ⊢ τ ∶ 𝓤 ℓ₁ → Γ ∷ τ ⊢ Id (↑ τ) (↑ a) # 0 ∶ 𝓤 ℓ₁
+   → Γ ∷ τ ∷ Id (↑ τ) (↑ a) # 0 ⊢ C₁ ≡ C₂ ∶ 𝓤 ℓ
+   → Γ ⊢ d₁ ≡ d₂ ∶ C₁ [/ refl (↑ τ) (↑ a) ] [/ a ] → Γ ⊢ p₁ ≡ p₂ ∶ Id τ a b
+    ---------------------------------------------------------------------------
+   → Γ ⊢ J C₁ d₁ p₁ ≡ J C₂ d₂ p₂ ∶ C₁ [/ ↑ p₁ ] [/ b ]
+| jβ : Γ ⊢ τ ∶ 𝓤 ℓ₁ → Γ ⊢ a ∶ τ
+    →  Γ ∷ τ ⊢ Id (↑ τ) (↑ a) # 0 ∶ 𝓤 ℓ₁
+    →  Γ ∷ τ ∷ Id (↑ τ) (↑ a) # 0 ⊢ C ∶ 𝓤 ℓ
+    →  Γ ⊢ d ∶ C [/ refl (↑ τ) (↑ a) ] [/ a ]
+     --------------------------------------------------------------
+    →  Γ ⊢ J C d (refl τ a) ≡ d ∶ C [/ refl (↑ τ) (↑ a) ] [/ a ]
 end
 end
 
--- A term is well-typed iff it is definitionally equal to itself.
-abbrev WfTm (Γ : Ctx n) (t τ : Tm n) : Prop := Γ ⊢ t ≡ t ∶ τ
+theorem DefEq.wf_left (h : Γ ⊢ t ≡ t' ∶ τ) : Γ ⊢ t ∶ τ :=
+  h.trans h.symm
 
-notation:40 Γ:41 "⊢" t:41 "∶" τ:41 => WfTm Γ t τ
-
--- Diagonalization: both sides of an equation are well-typed.
-theorem DefEq.wf_left (h : Γ ⊢ t ≡ t' ∶ τ) : Γ ⊢ t ∶ τ := h.trans h.symm
-
-theorem DefEq.wf_right (h : Γ ⊢ t ≡ t' ∶ τ) : Γ ⊢ t' ∶ τ := h.symm.trans h
+theorem DefEq.wf_right (h : Γ ⊢ t ≡ t' ∶ τ) : Γ ⊢ t' ∶ τ :=
+  h.symm.trans h
