SPos/Typing/Substitution.lean
@@ -51,7 +51,7 @@ theorem DefEq.subst (heq : Γ ⊢ t₁ ≡ t₂ ∶ τ) (hΔ : ⊢ Δ) (hσ : Su
       exact DefEq.lamη (DefEq.subst ht hΔ hσ)
   | .id hτeq haeq hbeq =>
       .id (DefEq.subst hτeq hΔ hσ) (DefEq.subst haeq hΔ hσ) (DefEq.subst hbeq hΔ hσ)
-  | .reflId hτeq haeq => .reflId (DefEq.subst hτeq hΔ hσ) (DefEq.subst haeq hΔ hσ)
+  | .refl hτeq haeq => .refl (DefEq.subst hτeq hΔ hσ) (DefEq.subst haeq hΔ hσ)
   | .j hτ hIdT hCeq hdeq hpeq => by
       have hτ' := DefEq.subst hτ hΔ hσ
       have hΔτ := hΔ.cons hτ'
